src/prop/FutureCertify.v
@@ -25,6 +25,7 @@ Require Import Thread.
 Require Import Cover.
 Require Import Mapping.
 Require Import Pred.
+Require Import Trace.
 Require Import MemoryProps.
 Require Import PFConsistent.
 Require Import PFConsistentStrong.
@@ -34,59 +35,6 @@ Set Implicit Arguments.
 Module FutureCertify.
   Section FutureCertify.
     Variable (lang: language).
-
-    Lemma future_memory_map
-          mem mem_cap mem_future times
-          (CAP: Memory.cap mem mem_cap)
-          (FUTURE: Memory.future_weak mem mem_future)
-          (CLOSED: Memory.closed mem):
-      exists (f: Loc.t -> Time.t -> Time.t -> Prop),
-        (<<IDENT: map_ident_in_memory f mem>>) /\
-        (<<MAPLT: mapping_map_lt f>>) /\
-        (<<MEMORY: memory_map f mem_cap mem_future>>) /\
-        (<<COMPLETE: forall loc to (IN: List.In to (times loc)),
-            exists fto, (<<MAPPED: f loc to fto>>)>>).
-    Proof.
-      exploit (choice (fun loc f =>
-                         (<<COMPLETE: forall to (IN: List.In to (Time.incr (Memory.max_ts loc mem)::(times loc))), exists fto, (<<MAPPED: f to fto>>)>>) /\
-                         (<<SAME: forall ts (TS: Time.le ts (Memory.max_ts loc mem)), f ts ts>>) /\
-                         (<<BOUND: forall to fto (MAPPED: f to fto) (TS: Time.lt (Memory.max_ts loc mem) to),
-                             (Time.lt (Time.join (Memory.max_ts loc mem_future) (Memory.max_ts loc mem)) fto)>>) /\
-                         (<<MAPLT: mapping_map_lt_loc f>>))).
-      { intros loc. hexploit shift_map_exists.
-        - eapply Time.join_r.
-        - eapply Time.incr_spec.
-        - i. des. exists f. esplits; eauto.
-          i. exploit BOUND; eauto. i. des. eapply x. }
-      intros [f FSPEC]. exists f.
-      assert (IDENT: map_ident_in_memory f mem).
-      { ii. specialize (FSPEC loc). des. eauto. }
-      splits; eauto.
-      - ii. specialize (FSPEC loc). des. eauto.
-      - econs.
-        + i. eapply Memory.cap_inv in GET; eauto. des; eauto.
-          dup GET. destruct msg; eauto. eapply Memory.future_weak_get1 in GET; eauto. des.
-          right. esplits; eauto.
-          * specialize (FSPEC loc). des. eapply SAME.
-            eapply Memory.max_ts_spec in GET0. des. auto.
-          * eapply map_ident_in_memory_closed_message; eauto.
-            inv CLOSED. eapply CLOSED0 in GET0. des. eauto.
-        + i. specialize (FSPEC loc). des.
-          exploit COMPLETE.
-          { ss. left. auto. } i. des.
-          exploit BOUND; eauto.
-          { eapply Time.incr_spec. } i.
-          left. esplits.
-          * eapply MAPPED.
-          * eapply Time.bot_spec.
-          * eapply Memory.max_ts_spec in GET. des.
-            etrans; eauto. etrans.
-            { eapply Time.join_l. }
-            { left. eapply x. }
-          * eapply map_ident_in_memory_bot; eauto.
-          * i. inv CLOSED. eapply memory_cap_covered; eauto.
-      - ii. specialize (FSPEC loc). des. eapply COMPLETE; ss; eauto.
-    Qed.
 
     Lemma cap_steps_current_steps
           th0 th1 mem1 sc1
@@ -108,17 +56,13 @@ Module FutureCertify.
     .
     Proof.
       eapply pred_steps_thread_steps in STEPS.
-      eapply pred_steps_traced_step in STEPS. des.
-      hexploit traced_times_list_exists; eauto. i. des.
-      exploit (@future_memory_map _ _ th0.(Thread.memory) times CAP); eauto.
-      { refl. } i. des.
       destruct th0, th1. ss.
-      hexploit traced_steps_map.
-      { eapply mapping_map_lt_map_le; eauto. }
-      { eapply map_ident_in_memory_bot; eauto. }
-      { eapply mapping_map_lt_map_eq; eauto. }
-      { eapply wf_time_mapped_mappable; eauto. }
-      { eauto. }
+      hexploit steps_map.
+      { eapply ident_map_le. }
+      { eapply ident_map_bot. }
+      { eapply ident_map_eq. }
+      { i. eapply ident_map_mappable_evt. }
+      { eapply STEPS. }
       { ss. }
       { ss. }
       { ss. }
@@ -128,28 +72,36 @@ Module FutureCertify.
       { eapply Memory.cap_closed; eauto. }
       { eauto. }
       { eapply Memory.max_concrete_timemap_closed; eauto. }
-      { eapply map_ident_in_memory_local; eauto. }
-      { eauto. }
-      { eapply mapping_map_lt_collapsable_unwritable. eauto. }
-      { eapply map_ident_in_memory_closed_timemap; eauto.
-        ss. eapply memory_concrete_le_closed_timemap; cycle 1.
-        - eapply Memory.max_concrete_timemap_closed; eauto.
-        - ii. eapply Memory.cap_inv in GET; eauto. des; clarify. }
+      { eapply map_ident_in_memory_local; eauto; ss.
+        eapply ident_map_lt.
+      }
+      { econs.
+        { i. destruct msg as [val released|]; auto. right.
+          exists to, from, (Message.concrete val released), (Message.concrete val released).
+          eapply Memory.cap_inv in GET; eauto. des; ss. esplits; eauto.
+          { refl. }
+          { eapply ident_map_message. }
+          { refl. }
+        }
+        { i. eapply CAP in GET. left. exists fto, ffrom, fto, ffrom. splits; ss.
+          { refl. }
+          { refl. }
+          { i. econs; eauto. }
+        }
+      }
+      { eapply mapping_map_lt_collapsable_unwritable. eapply ident_map_lt. }
+      { eapply ident_map_timemap. }
       { eapply Memory.max_concrete_timemap_spec; eauto.
         eapply Memory.cap_closed_timemap; eauto. }
-      i. des. eapply pred_steps_traced_step2 in STEPS.
-      - exists flc1, fsc1, fmem1. split.
-        + eapply thread_steps_pred_steps; eauto.
-        + inv LOCAL0. eapply promise_consistent_mon; cycle 1; eauto.
-          { refl. }
-          eapply promise_consistent_map; eauto.
-          { eapply mapping_map_lt_map_le; eauto. }
-          { eapply mapping_map_lt_map_eq; eauto. }
-      - apply List.Forall_forall. ii.
-        eapply list_Forall2_in in H; eauto. des. split.
-        { instantiate (1:=fun _ => True). ss. }
-        eapply List.Forall_forall in EVENTS; eauto. des.
-        destruct a, x. ss. inv EVENT; auto.
+      { instantiate (1:=fun _ => True). ss. }
+      i. des. esplits.
+      { eapply rtc_implies; try apply STEP. i. inv H. inv TSTEP. econs; eauto. }
+      { inv LOCAL0. eapply promise_consistent_mon; cycle 1; eauto.
+        { refl. }
+        eapply promise_consistent_map; eauto.
+        { eapply ident_map_le; eauto. }
+        { eapply ident_map_eq; eauto. }
+      }
     Qed.
 
     Definition future_certify lang (e:Thread.t lang): Prop :=
@@ -172,79 +124,13 @@ Module FutureCertify.
           (CONSISTENT: @Thread.consistent lang e):
       future_certify e.
     Proof.
-      eapply consistent_pf_consistent in CONSISTENT; eauto.
-      eapply pf_consistent_pf_consistent_strong in CONSISTENT; eauto.
-      ii. hexploit Memory.cap_exists.
-      { eapply MEMORY. } i. des.
-      exploit CONSISTENT; eauto.
-      instantiate (1:=TimeMap.bot). i. des.
-      eapply pred_steps_traced_step in STEPS0. des.
-      eapply pred_steps_traced_step in STEPS1. des.
-
-      hexploit traced_times_list_exists.
-      { eapply traced_step_trans.
-        - eapply STEPS.
-        - eapply STEPS0. } i. des.
-      hexploit (future_memory_map times CAP FUTURE); eauto. i. des.
-
-      destruct e1, e2.
-      hexploit traced_steps_map.
-      { eapply mapping_map_lt_map_le; eauto. }
-      { eapply map_ident_in_memory_bot; eauto. }
-      { eapply mapping_map_lt_map_eq; eauto. }
-      { eapply wf_time_mapped_mappable; eauto. }
-      { eapply traced_step_trans; eauto. }
-      { eauto. }
-      { eauto. }
-      { eauto. }
-      { eapply Local.cap_wf; eauto. }
-      { eapply WF. }
-      { eauto. }
-      { eapply Memory.cap_closed; eauto. }
-      { eapply Memory.closed_timemap_bot. inv MEM. auto. }
-      { eapply Memory.closed_timemap_bot.
-        eapply Memory.cap_closed in MEMORY; eauto. inv MEMORY. auto. }
-      { eapply map_ident_in_memory_local; eauto. }
-      { eauto. }
-      { eapply mapping_map_lt_collapsable_unwritable. eauto. }
-      { eapply timemap_bot_map. eapply map_ident_in_memory_bot; eauto. }
-      { refl. }
-      i. des.
-      hexploit no_sc_any_sc_traced.
-      { eapply STEPS1. }
-      { eauto. }
-      { eauto. }
-      { eauto. }
-      { ii. eapply list_Forall2_in in IN; eauto. des.
-        eapply List.in_app_or in IN0. des.
-        + eapply List.Forall_forall in EVENTS; eauto. des.
-          destruct a, e0. ss. inv EVENT; ss.
-        + eapply List.Forall_forall in EVENTS0; eauto. des.
-          destruct a, e0. ss. inv EVENT; ss. }
-      i. des. eapply pred_steps_traced_step2 in STEPS2.
-      - unguard. des; ss.
-        + left. unfold Thread.steps_failure. esplits.
-          * eapply thread_steps_pred_steps. eapply STEPS2.
-          * econs 2. econs; eauto. econs. econs.
-            inv LOCAL0. inv LOCAL1. destruct local0.
-            eapply promise_consistent_mon.
-            { eapply promise_consistent_map; eauto.
-              - eapply mapping_map_lt_map_le; eauto.
-              - eapply mapping_map_lt_map_eq; eauto. }
-            { auto. }
-            { refl. }
-        + right. esplits.
-          * eapply thread_steps_pred_steps. eapply STEPS2.
-          * ss. inv LOCAL0. rewrite PROMISES in *.
-            eapply bot_promises_map in PROMISES0. auto.
-      - apply List.Forall_forall. ii.
-        eapply list_Forall2_in in H; eauto. des. split.
-        { instantiate (1:=fun _ => True). ss. }
-        eapply List.in_app_or in IN. des.
-        + eapply List.Forall_forall in EVENTS; eauto. des.
-          destruct a, x. ss. inv EVENT; auto.
-        + eapply List.Forall_forall in EVENTS0; eauto. des.
-          destruct a, x. ss. inv EVENT; auto.
+      eapply consistent_pf_consistent_super_strong in CONSISTENT; eauto. des.
+      ii. exploit (CONSISTENT0 mem1 TimeMap.bot sc1); eauto. i. des.
+      eapply Trace.silent_steps_tau_steps in STEPS; cycle 1.
+      { eapply List.Forall_impl; eauto. i. ss. des. auto. }
+      unguard. des.
+      { left. unfold Thread.steps_failure. destruct e1. ss. esplits; eauto. }
+      { right. esplits; eauto. }
     Qed.
 
     Lemma future_consistent
