src/prop/Pred.v
@@ -22,6 +22,7 @@ Require Import Thread.
 Require Import Configuration.
 Require Import Progress.
 Require Import Behavior.
+Require Import Trace.
 
 Set Implicit Arguments.
 
@@ -241,125 +242,6 @@ Section PredStep.
   | pred_step_intro (STEP : Thread.step_allpf e e1 e2) (SAT : P e)
   .
 
-  Inductive traced_step lang: list (ThreadEvent.t * Memory.t) -> (Thread.t lang) -> (Thread.t lang) -> Prop :=
-  | traced_step_refl
-      th0
-    :
-      traced_step [] th0 th0
-  | traced_step_step
-      th0 th1 th2 hde hdm tl
-      (HD: Thread.step_allpf hde th0 th1)
-      (TL: traced_step tl th1 th2)
-      (MEM: hdm = th0.(Thread.memory))
-    :
-      traced_step ((hde, hdm)::tl) th0 th2
-  .
-
-  Inductive traced_step_n1 lang: list (ThreadEvent.t * Memory.t) -> (Thread.t lang) -> (Thread.t lang) -> Prop :=
-  | traced_step_n1_refl
-      th0
-    :
-      traced_step_n1 [] th0 th0
-  | traced_step_n1_step
-      th0 th1 th2 hds tle tlm
-      (HD: traced_step_n1 hds th0 th1)
-      (TL: Thread.step_allpf tle th1 th2)
-      (MEM: tlm = th1.(Thread.memory))
-    :
-      traced_step_n1 (hds++[(tle, tlm)]) th0 th2
-  .
-
-  Lemma traced_step_n1_one lang (th0 th1: Thread.t lang) e
-        (STEP: Thread.step_allpf e th0 th1)
-    :
-      traced_step_n1 [(e, th0.(Thread.memory))] th0 th1.
-  Proof.
-    erewrite <- List.app_nil_l at 1. econs; eauto. econs 1.
-  Qed.
-
-  Lemma traced_step_n1_trans lang (th0 th1 th2: Thread.t lang) tr0 tr1
-        (STEPS0: traced_step_n1 tr0 th0 th1)
-        (STEPS1: traced_step_n1 tr1 th1 th2)
-    :
-      traced_step_n1 (tr0 ++ tr1) th0 th2.
-  Proof.
-    ginduction STEPS1; i; ss.
-    - erewrite List.app_nil_r. auto.
-    - rewrite List.app_assoc. econs; eauto.
-  Qed.
-
-  Lemma traced_step_one lang (th0 th1: Thread.t lang) e
-        (STEP: Thread.step_allpf e th0 th1)
-    :
-      traced_step [(e, th0.(Thread.memory))] th0 th1.
-  Proof.
-    econs 2; eauto. econs 1.
-  Qed.
-
-  Lemma traced_step_trans lang (th0 th1 th2: Thread.t lang) tr0 tr1
-        (STEPS0: traced_step tr0 th0 th1)
-        (STEPS1: traced_step tr1 th1 th2)
-    :
-      traced_step (tr0 ++ tr1) th0 th2.
-  Proof.
-    ginduction STEPS0; i; ss.
-    econs; eauto.
-  Qed.
-
-  Lemma traced_step_equivalent lang (th0 th1: Thread.t lang) tr
-    :
-        traced_step tr th0 th1 <-> traced_step_n1 tr th0 th1.
-  Proof.
-    split; intros STEP.
-    - ginduction STEP.
-      + econs.
-      + exploit traced_step_n1_trans.
-        * apply traced_step_n1_one; eauto.
-        * eauto.
-        * ss. clarify.
-    - ginduction STEP.
-      + econs.
-      + eapply traced_step_trans; eauto.
-        clarify. eapply traced_step_one; eauto.
-  Qed.
-
-  Lemma traced_step_separate lang (th0 th2: Thread.t lang) tr0 tr1
-        (STEPS: traced_step (tr0++tr1) th0 th2)
-    :
-      exists th1,
-        (<<STEPS0: traced_step tr0 th0 th1>>) /\
-        (<<STEPS1: traced_step tr1 th1 th2>>).
-  Proof.
-    ginduction tr0; i; ss.
-    - exists th0. splits; ss. econs.
-    - inv STEPS. eapply IHtr0 in TL. des.
-      exists th1. splits; ss.
-      econs; eauto.
-  Qed.
-
-  Lemma traced_step_in P lang (th0 th1: Thread.t lang) tr e m
-        (STEPS: traced_step tr th0 th1)
-        (IN: List.In (e, m) tr)
-        (PRED: List.Forall P tr)
-    :
-      exists th' th'' tr0 tr1,
-        (<<STEPS0: traced_step tr0 th0 th'>>) /\
-        (<<STEP: Thread.step_allpf e th' th''>>) /\
-        (<<MEM: m = th'.(Thread.memory)>>) /\
-        (<<STEPS1: traced_step tr1 th'' th1>>) /\
-        (<<TRACES: tr = tr0 ++ [(e, m)] ++ tr1>>) /\
-        (<<SAT: P (e, m)>>).
-  Proof.
-    ginduction STEPS; i; ss. inv PRED. des.
-    - clarify. exists th0, th1. esplits; eauto.
-      + econs 1.
-      + ss.
-    - exploit IHSTEPS; eauto. i. des.
-      esplits; eauto.
-      + econs 2; eauto.
-      + clarify.
-  Qed.
-
   Lemma pred_step_program_step P:
         @pred_step P <4= @Thread.step_allpf.
   Proof.
@@ -437,36 +319,36 @@ Section PredStep.
       eapply no_promise_program_step; eauto.
   Qed.
 
-  Lemma pred_steps_traced_step P lang
+  Lemma pred_steps_trace_steps P lang
         th0 th1
     :
       rtc (tau (@pred_step P lang)) th0 th1 <->
       exists tr,
-        (<<STEPS: traced_step tr th0 th1>>) /\
-        (<<EVENTS: List.Forall (fun em => <<SAT: P (fst em)>> /\ <<TAU: ThreadEvent.get_machine_event (fst em) = MachineEvent.silent>>) tr >>)
+        (<<STEPS: Trace.steps tr th0 th1>>) /\
+        (<<EVENTS: List.Forall (fun em => <<SAT: P (snd em)>> /\ <<TAU: ThreadEvent.get_machine_event (snd em) = MachineEvent.silent>>) tr >>)
   .
   Proof.
     split; i.
     - ginduction H; i.
-      + exists []. splits; eauto. econs 1.
-      + des. inv H. inv TSTEP. exists ((e, x.(Thread.memory))::tr). splits.
-        * econs; eauto.
+      + exists []. splits; eauto.
+      + des. inv H. inv TSTEP. exists ((x, e)::tr). splits.
+        * inv STEP. econs; eauto.
         * i. ss. des; clarify. eauto.
     - des. ginduction STEPS; i.
       + refl.
-      + inv EVENTS. des. econs.
-        * econs; eauto. econs; eauto.
+      + inv EVENTS; ss. clarify. des. econs.
+        * econs; eauto. econs; eauto. econs; eauto.
         * eauto.
   Qed.
 
-  Lemma pred_steps_traced_step2 P lang
+  Lemma pred_steps_trace_steps2 P lang
         th0 th1 tr
-        (STEPS: traced_step tr th0 th1)
-        (EVENTS: List.Forall (fun em => <<SAT: P (fst em)>> /\ <<TAU: ThreadEvent.get_machine_event (fst em) = MachineEvent.silent>>) tr)
+        (STEPS: Trace.steps tr th0 th1)
+        (EVENTS: List.Forall (fun em => <<SAT: P (snd em)>> /\ <<TAU: ThreadEvent.get_machine_event (snd em) = MachineEvent.silent>>) tr)
   :
     rtc (tau (@pred_step P lang)) th0 th1.
   Proof.
-    eapply pred_steps_traced_step; eauto.
+    eapply pred_steps_trace_steps; eauto.
   Qed.
 
   Lemma pf_step_promise_free_step lang:
@@ -510,44 +392,39 @@ Section PredStep.
   Definition same_machine_event e_src e_tgt :=
     ThreadEvent.get_machine_event e_src = ThreadEvent.get_machine_event e_tgt.
 
-  Lemma step_times_list_exists lang (th0 th1: Thread.t lang) e
-        (STEP: Thread.step_allpf e th0 th1)
+  Lemma event_times_list_exists
+        e
+    :
+      exists (times: Loc.t -> list Time.t),
+        (<<EVT: wf_time_evt (fun loc ts => List.In ts (times loc)) e >>).
+  Proof.
+    destruct e; ss; try by (exists (fun _ => []); splits; auto).
+    { exists (fun loc' => if Loc.eq_dec loc' loc then [from; to] else []).
+      des_ifs; ss; auto. }
+    { exists (fun loc' => if Loc.eq_dec loc' loc then [from; to] else []).
+      des_ifs; ss; auto. }
+    { exists (fun loc' => if Loc.eq_dec loc' loc then [tsr; tsw] else []).
+      des_ifs; ss; auto. }
+  Qed.
+
+  Lemma step_times_list_exists lang (th0 th1: Thread.t lang) e pf
+        (STEP: Thread.step pf e th0 th1)
     :
       exists (times: Loc.t -> list Time.t),
         (<<WFTIME: wf_time_evt (fun loc to => List.In to (times loc)) e>>).
   Proof.
-    destruct e.
-    - exists (fun l => if Loc.eq_dec l loc then
-                         [from; to] else []).
-      econs; eauto.
-      + ss. splits; auto; des_ifs; ss; eauto.
-      + ss. splits; auto; des_ifs; ss; eauto.
-    - exists (fun _ => []). econs; eauto.
-    - exists (fun _ => []). econs; eauto.
-    - exists (fun l => if Loc.eq_dec l loc then
-                         [from; to] else []).
-      econs; eauto.
-      + ss. splits; auto; des_ifs; ss; eauto.
-      + ss. splits; auto; des_ifs; ss; eauto.
-    - exists (fun l => if Loc.eq_dec l loc then
-                         [tsr; tsw] else []).
-      econs; eauto.
-      + ss. splits; auto; des_ifs; ss; eauto.
-      + ss. splits; auto; des_ifs; ss; eauto.
-    - exists (fun _ => []). econs; eauto.
-    - exists (fun _ => []). econs; eauto.
-    - exists (fun _ => []). econs; eauto.
+    exploit event_times_list_exists; eauto.
   Qed.
 
-  Lemma traced_times_list_exists lang (th0 th1: Thread.t lang) tr
-        (STEPS: traced_step tr th0 th1)
+  Lemma trace_times_list_exists lang (th0 th1: Thread.t lang) tr
+        (STEPS: Trace.steps tr th0 th1)
     :
       exists (times: Loc.t -> list Time.t),
-        (<<WFTIME: List.Forall (fun em => wf_time_evt (fun loc to => List.In to (times loc)) (fst em)) tr>>).
+        (<<WFTIME: List.Forall (fun em => wf_time_evt (fun loc to => List.In to (times loc)) (snd em)) tr>>).
   Proof.
     ginduction STEPS.
     - exists (fun _ => []). econs.
-    - des. eapply step_times_list_exists in HD. des.
+    - des. clarify. eapply step_times_list_exists in STEP. des.
       exists (fun loc => (times0 loc ++ times loc)). econs.
       + eapply wf_time_evt_mon; eauto.
         i. ss. eapply List.in_or_app; eauto.
@@ -565,25 +442,5 @@ Section PredStep.
     :
       opt_pred_step P e t0 t1.
   Hint Constructors opt_pred_step.
-
-  Lemma traced_step_future lang
-        (e1 e2: Thread.t lang) tr
-        (STEP: traced_step tr e1 e2)
-        (WF1: Local.wf e1.(Thread.local) e1.(Thread.memory))
-        (SC1: Memory.closed_timemap e1.(Thread.sc) e1.(Thread.memory))
-        (CLOSED1: Memory.closed e1.(Thread.memory)):
-    (<<WF2: Local.wf e2.(Thread.local) e2.(Thread.memory)>>) /\
-    (<<SC2: Memory.closed_timemap e2.(Thread.sc) e2.(Thread.memory)>>) /\
-    (<<CLOSED2: Memory.closed e2.(Thread.memory)>>) /\
-    (<<TVIEW_FUTURE: TView.le e1.(Thread.local).(Local.tview) e2.(Thread.local).(Local.tview)>>) /\
-    (<<SC_FUTURE: TimeMap.le e1.(Thread.sc) e2.(Thread.sc)>>) /\
-    (<<MEM_FUTURE: Memory.future e1.(Thread.memory) e2.(Thread.memory)>>).
-  Proof.
-    revert WF1. induction STEP.
-    - i. splits; ss; refl.
-    - i. subst. inv HD. exploit Thread.step_future; eauto. i. des.
-      exploit IHSTEP; eauto. i. des.
-      splits; ss; etrans; eauto.
-  Qed.
 
 End PredStep.
